try to fix the proofs for programs returning any [Type] instead of [Set]
still stuck on a universe inconsistency that i don't know how to fix
(which is the original reason we were returning [Set] instead of [Type]):

  % make proof
  ...
  "coqc"  -q  -R "coqproof" Fscq   coqproof/BasicProg
  Identifier 'If' now a keyword
  File "./coqproof/BasicProg.v", line 193, characters 0-4:
  Error: Illegal application:
  The term "fun A A0 : Type => A -> A0" of type "Type -> Type -> Type"
  cannot be applied to the terms
   "L" : "Type"
   "prog T" : "Type"
  The 2nd term has type "Type@{max(Set, Fscq.BasicProg.80)}"
  which should be coercible to "Type@{Fscq.BasicProg.227}".

src/Hoare.v
@@ -7,9 +7,9 @@ Set Implicit Arguments.
 
 (** ** Hoare logic *)
 
-Definition donecond (T: Set) := T -> @mem valu -> Prop.
+Definition donecond (T: Type) := T -> @mem valu -> Prop.
 
-Definition corr2 (T: Set) (pre: donecond T -> pred -> pred) (p: prog T) :=
+Definition corr2 (T: Type) (pre: donecond T -> pred -> pred) (p: prog T) :=
   forall done crash m out, pre done crash m
   -> exec m p out
   -> (exists m' v, out = Finished m' v /\ done v m') \/
@@ -19,7 +19,7 @@ Notation "{{ pre }} p" := (corr2 pre%pred p)
   (at level 0, p at level 60).
 
 
-Definition corr3 (TF TR: Set) (pre: donecond TF -> donecond TR -> pred)
+Definition corr3 (TF TR: Type) (pre: donecond TF -> donecond TR -> pred)
                  (p1: prog TF) (p2: prog TR) :=
   forall done crashdone m out, pre done crashdone m
   -> exec_recover m p1 p2 out
@@ -203,7 +203,7 @@ Proof.
 Qed.
 
 
-Instance corr2_proper {T : Set} :
+Instance corr2_proper {T : Type} :
   Proper (pointwise_relation (donecond T) (pointwise_relation pred piff)
           ==> eq ==> iff) (@corr2 T).
 Proof.
@@ -211,7 +211,7 @@ Proof.
   split; intros; eapply pimpl_ok2; try eassumption; apply Hab.
 Qed.
 
-Instance corr3_proper {T R : Set} :
+Instance corr3_proper {T R : Type} :
   Proper (pointwise_relation (donecond T) (pointwise_relation (donecond R) piff)
           ==> eq ==> eq ==> iff) (@corr3 T R).
 Proof.
